\documentclass[12pt]{article}
\usepackage[utf8]{inputenc}
\usepackage{amsthm}
\usepackage{amsmath}
\usepackage{amssymb}
\begin{document}

\begin{align*}
	&\text{Forecast equation: } \hat{y}_{t+h|t} = l_t \\
	&\text{Smoothing equation: } l_t = \alpha y_t + (1-\alpha) l_{t-1}
\end{align*}

\begin{align*}
	&\text{Forecast equation: } \hat{y}_{t+h|t} = l_t + b_t h\\
	&\text{Level equation: } l_t = \alpha y_t + (1-\alpha) (l_{t-1} + b_{t-1}) \\
	&\text{Trend equation: } b_t = \beta^*(l_t - l_{t-1}) + (1-\beta^*) b_{t-1}
\end{align*}

\begin{align*}
	&\text{Forecast equation: } \hat{y}_{t+h|t} = l_t + b_t (\phi + \phi^2 + \ldots + \phi^h)\\
	&\text{Level equation: } l_t = \alpha y_t + (1-\alpha) (l_{t-1} + \phi b_{t-1}) \\
	&\text{Trend equation: } b_t = \beta^*(l_t - l_{t-1}) + (1-\beta^*) \phi b_{t-1}
\end{align*}

\begin{align*}
	\hat{y}_{t+h|t} = l_t + b_t \phi \sum_{n=0}^h \phi^n \underset{h\rightarrow \infty}{\longrightarrow} l_t + \frac{\phi}{1-\phi} b_t
\end{align*}


\begin{align*}
	&\text{Forecast equation: } \hat{y}_{t+h|t} = l_t + h b_t + s_{t+h-m(k+1)} \\
	&\text{Level equation: } l_t = \alpha (y_t - s_{t-m}) + (1-\alpha) (l_{t-1} + b_{t-1}) \\
	&\text{Trend equation: } b_t = \beta^*(l_t - l_{t-1}) + (1-\beta^*) b_{t-1} \\
	&\text{Seasonal equation: } s_t = \gamma^*(y_t - l_t) + (1-\gamma^*) s_{t-m}
\end{align*}

\end{document}
